crypto_examples/mulntt_ct/mulntt_ct.dfy
@@ -1,4 +1,5 @@
 include "nth_root.dfy"
+include "mulntt_ct_rec.dfy"
 
 module ntt {
     import opened Seq
@@ -9,43 +10,141 @@ module ntt {
 
     import opened pows_of_2
     import opened omegas
+
+    import opened mulntt_ct_rec
     // import opened ntt_recs
     // import opened rindex
     // import opened bins
     // import opened polys
 
+    function method block_count(m: pow2_t): nat
+        requires 0 <= m.exp <= LOGN;
+    {
+        pow2_div(pow2(LOGN), m).full
+    }
+
+    lemma block_count_product_lemma(m: pow2_t)
+        requires 0 <= m.exp <= LOGN;
+        ensures block_count(m) * m.full == N;
+    {
+        Nth_root_lemma();
+    }
+
+    lemma block_count_half_lemma(m: pow2_t)
+        requires 1 <= m.exp <= LOGN;
+        ensures block_count(pow2_half(m)) == block_count(m) * 2;
+    {
+        Nth_root_lemma();
+        var left := pow2_div(pow2(LOGN), pow2_half(m));
+        assert left.full * (m.full / 2) == N;
+        var right := pow2_div(pow2(LOGN), m);
+        var half := m.full / 2;
+        pow2_basics(m);
+
+        calc == {
+            left.full * half;
+            left.full * (m.full / 2);
+            right.full * (2 * half);
+            {
+                LemmaMulIsAssociativeAuto();
+            }
+            (right.full * 2) * half;
+        }
+        LemmaMulEqualityConverse(half, left.full, right.full * 2);
+    }
+
     type n_sized = s: seq<elem>
         | |s| == N == pow2(LOGN).full witness *
 
-    function method A(): seq<elem>
-        ensures |A()| == N == pow2(LOGN).full;
+    function method A(): n_sized
 
-    function method P(): seq<elem>
-        ensures |P()| == N == pow2(LOGN).full;
+    function method P(): n_sized
 
-    method slice_loop(u: nat,
-        d: pow2_t,
-        w: elem,
-        ghost j: nat,
-        ghost blocks: seq<seq<elem>>)
-        requires |blocks| == d.full;
+    lemma A_table_index_bounded_lemma(s: nat, d: pow2_t, j: nat, t: pow2_t)
+        requires 0 <= d.exp < LOGN;
+        requires 0 <= t.exp < LOGN;
+        requires block_count(t) == 2 * d.full;
+        // requires block_count(pow2_double(t)) == d.full;
+        requires j < t.full;
+        requires s < (2 * d.full) * j + d.full;
+        ensures s + d.full < N;
     {
-        var s := u;
+        assume false;
+        // block_count_product_lemma(t);
+        // assert block_count(t) * t.full == N;
+    }
 
-        while (s < u + d.full)
+    datatype slice_loop_view = slice_loop_view(
+        lower: lpolys,
+        higher: lpolys)
+    {
+        predicate slice_view_wf()
         {
-            ghost var b_idx := s - u;
-
-            var oi := s + d.full;
-            var ei := s;
-
-            s := s + 1;
-
-            // blocks[b_idx := blocks[b_idx]];
+            && higher.level_wf()
+            && lower.level_wf()
+            && 1 <= higher.bsize.exp <= LOGN
+            && higher.build_smaller_level() == lower
         }
     }
 
-    lemma P_table_index_bounded(t: pow2_t, j: nat)
+    // predicate slice_loop_inv()
+
+    function bit_rev_int(j: nat, bound: pow2_t): nat
+
+    method slice_loop(
+        a: n_sized,
+        u: nat,
+        d: pow2_t,
+        w: elem,
+        ghost j: nat,
+        ghost t: pow2_t)
+        // ghost sv: slice_loop_view)
+
+    returns (new_a: n_sized)
+    
+    // ghost new_blocks: seq<seq<elem>>)
+        // requires |blocks| == d.full;
+        requires 0 <= t.exp < LOGN;
+        requires 0 <= d.exp < LOGN;
+
+        requires 2 * d.full * bit_rev_int(j, t) >= 0;
+
+        requires block_count(t) == 2 * d.full;
+        // d blocks, each of 2t size 
+        // requires block_count(pow2_double(t)) == d.full;
+        requires j < t.full;
+        requires u == (2 * d.full) * j;
+        // requires t.exp == 0 ==> a == A();
+
+        // ensures |new_blocks| == d.full;
+    {
+        var s := u;
+        // new_blocks := blocks;
+        new_a := a;
+
+        assume w == modpow(PSI, 2 * d.full * bit_rev_int(j, t) + d.full);
+
+        while (s < u + d.full)
+            // invariant |new_blocks| == |blocks|;
+            // invariant 
+        {
+            A_table_index_bounded_lemma(s, d, j, t);
+            ghost var b_idx := s - u;
+            var e := a[s];
+            var o := a[s + d.full];
+
+            // assume e == 
+
+            var x := modmul(o, w);
+            new_a := new_a[s+d.full := modsub(e, x)];
+            new_a := new_a[s := modadd(e, x)];
+
+            s := s + 1;
+            // new_blocks := new_blocks[b_idx := blocks[b_idx]];
+        }
+    }
+
+    lemma P_table_index_bounded_lemma(t: pow2_t, j: nat)
         requires t.exp < LOGN;
         requires j < t.full;
         ensures t.full + j < N;
@@ -53,56 +152,65 @@ module ntt {
         assume false;
     }
 
-    method level_loop(t: pow2_t, d: pow2_t)
-        requires t.exp < LOGN;
-        requires d.exp + 1 + t.exp == LOGN;
-    {
-        var j := 0;
-        var u := 0;
+    // method level_loop(a: n_sized, t: pow2_t, d: pow2_t)
+    //     requires t.exp < LOGN;
+    //     requires d.exp + 1 + t.exp == LOGN;
+    //     requires block_count(pow2_double(t)) == d.full;
+    //     requires block_count(t) == 2 * d.full;
+    // {
+    //     var j := 0;
+    //     var u := 0;
 
-        ghost var blocks := seq(d.full, n requires 0 <= n < d.full => []);
+    //     ghost var blocks := seq(d.full, n requires 0 <= n < d.full => []);
 
-        while (j < t.full)
-            invariant 0 <= u == (2 * d.full) * j;
-        {
-            P_table_index_bounded(t, j);
-            var w := P()[t.full + j]; // psi_t * w_t^bitrev(j)
+    //     while (j < t.full)
+    //         invariant 0 <= u == (2 * d.full) * j;
+    //         invariant |blocks| == d.full;
+    //     {
+    //         P_table_index_bounded_lemma(t, j);
+    //         var w := P()[t.full + j]; // psi_t * w_t^bitrev(j)
 
-            ghost var prev_u := u;
-            ghost var prev_j := j;
+    //         ghost var prev_u := u;
+    //         ghost var prev_j := j;
 
-            slice_loop(u, d, w, j, blocks);
-            j := j + 1;
-            u := u + 2 * d.full;
+    //         blocks := slice_loop(u, d, w, j, t, blocks);
+    //         j := j + 1;
+    //         u := u + 2 * d.full;
 
-            calc == {
-                u;
-                prev_u + 2 * d.full;
-                2 * d.full * prev_j + 2 * d.full;
-                {
-                    LemmaMulIsDistributive(2 * d.full, prev_j, 1);
-                }
-                (2 * d.full) * (prev_j + 1);
-            }
-        }
-    }
+    //         calc == {
+    //             u;
+    //             prev_u + 2 * d.full;
+    //             2 * d.full * prev_j + 2 * d.full;
+    //             {
+    //                 LemmaMulIsDistributive(2 * d.full, prev_j, 1);
+    //             }
+    //             (2 * d.full) * (prev_j + 1);
+    //         }
+    //     }
+    // }
 
-    method mulntt_ct()
-    {
-        var d := pow2(LOGN);
-        var t := pow2(0);
-        Nth_root_lemma();
+    // method mulntt_ct()
+    // {
+    //     var d := pow2(LOGN);
+    //     var t := pow2(0);
+    //     Nth_root_lemma();
 
-        while (t.full < N)
-            invariant d.exp + t.exp == LOGN;
-            invariant t.exp <= LOGN;
-        {
-            d := pow2_half(d);
+    //     while (t.full < N)
+    //         invariant d.exp + t.exp == LOGN;
+    //         invariant t.exp <= LOGN;
+    //         invariant block_count(t) == d.full;
+    //     {
+    //         d := pow2_half(d);
 
-            // assert d.exp + 1 + t.exp == LOGN;
-            // assume d.full * 2 * t.full == N;
-            level_loop(t, d);
-            t := pow2_double(t);
-        }
-    }
+    //         block_count_half_lemma(pow2_double(t));
+    //         // assert block_count(pow2_double(t)) == d.full;
+    //         // assert block_count(t) == 2 * d.full;
+
+    //         // assert d.exp + 1 + t.exp == LOGN;
+    //         // assume d.full * 2 * t.full == N;
+    //         level_loop(t, d);
+    //         t := pow2_double(t);
+    //         // block_count_half_lemma(t);
+    //     }
+    // }
 }
