crypto_examples/mulntt_ct/mulntt_ct_rec.dfy
@@ -1,0 +1,135 @@
+include "nth_root.dfy"
+
+module mulntt_ct_rec {
+    import opened Seq
+    import opened Power
+    import opened Power2
+    import opened DivMod
+    import opened Mul
+
+    import opened pows_of_2
+    import opened omegas
+
+    // function method A(): seq<elem>
+    //     ensures |A()| == N == pow2(LOGN).full;
+
+    function method {:opaque} even_indexed_items<T>(a: seq<T>, len: pow2_t): seq<T>
+        requires |a| == len.full;
+    {
+        pow2_basics(len);
+        seq(len.full/2, n requires 0 <= n < len.full/2 => a[n * 2])
+    }
+
+    function method {:opaque} odd_indexed_items<T>(a: seq<T>, len: pow2_t): seq<T>
+        requires |a| == len.full;
+    {
+        pow2_basics(len);
+        seq(len.full/2, n requires 0 <= n < len.full/2 => a[n * 2 + 1])
+    }
+
+    function method block_count(m: pow2_t): nat
+        requires 0 <= m.exp <= LOGN;
+    {
+        pow2_div(pow2(LOGN), m).full
+    }
+
+    lemma block_count_half_lemma(m: pow2_t)
+        requires 1 <= m.exp <= LOGN;
+        ensures block_count(pow2_half(m)) == block_count(m) * 2;
+    {
+        Nth_root_lemma();
+        var left := pow2_div(pow2(LOGN), pow2_half(m));
+        assert left.full * (m.full / 2) == N;
+        var right := pow2_div(pow2(LOGN), m);
+        var half := m.full / 2;
+        pow2_basics(m);
+
+        calc == {
+            left.full * half;
+            left.full * (m.full / 2);
+            right.full * (2 * half);
+            {
+                LemmaMulIsAssociativeAuto();
+            }
+            (right.full * 2) * half;
+        }
+        LemmaMulEqualityConverse(half, left.full, right.full * 2);
+    }
+
+    datatype lpolys = lpolys_cons(blocks: seq<seq<elem>>, bsize: pow2_t)
+    {
+        predicate {:opaque} level_wf()
+        {
+            && (forall i: nat | i < |blocks| :: |blocks[i]| == bsize.full)
+            && 0 <= bsize.exp <= LOGN
+            && block_count(bsize) == |blocks|
+        }
+
+        function method {:opaque} build_smaller_level(): (lps: lpolys)
+            requires level_wf();
+            requires 1 <= bsize.exp <= LOGN;
+            ensures lps.level_wf();
+            ensures lps.bsize == pow2_half(bsize);
+        {
+            reveal level_wf();
+            pow2_basics(bsize);
+            block_count_half_lemma(bsize);
+            var new_size := pow2_half(bsize);
+            var new_count := |blocks| * 2;
+            var new_blocks := seq(new_count, n requires 0 <= n < new_count => 
+                if n % 2 == 0 then even_indexed_items(blocks[n/2], bsize)
+                else odd_indexed_items(blocks[n/2], bsize));
+            var l := lpolys_cons(new_blocks, new_size);
+            assert l.level_wf() by {
+                reveal l.level_wf();
+            }
+            l
+        }
+
+        // lemma base_level_correct()
+        //     requires blocks == [A()];
+        //     requires bsize.exp == LOGN;
+        //     ensures level_wf();
+        // {
+        //     reveal level_wf();
+        //     Nth_root_lemma();
+        //     assert bsize.full == N;
+        // }
+
+        lemma level_index_correspondence_lemma(i: nat, sl: lpolys)
+            requires level_wf();
+            requires 1 <= bsize.exp <= LOGN;
+            requires sl == build_smaller_level();
+            requires i < |blocks|;
+            ensures |blocks[i]| == bsize.full;
+            ensures 2 * i + 1 < |sl.blocks|;
+            ensures even_indexed_items(blocks[i], bsize) == sl.blocks[2 * i];
+            ensures odd_indexed_items(blocks[i], bsize) == sl.blocks[2 * i + 1];
+        {
+            reveal level_wf();
+            reveal build_smaller_level();
+            reveal sl.level_wf();
+        }
+    }
+
+    // function method build_lpolys(bsize: pow2_t): (lps: lpolys)
+    //     requires bsize.exp <= LOGN;
+    //     ensures lps.level_wf();
+    //     ensures lps.bsize == bsize;
+    //     decreases LOGN - bsize.exp;
+    // {
+    //     if bsize.exp == LOGN then
+    //         var l := lpolys_cons([A()], bsize);
+    //         l.base_level_correct();
+    //         l
+    //     else
+    //         var prev := build_lpolys(pow2_double(bsize));
+    //         // assert 1 <= pow2_double(bsize).exp <= LOGN;
+    //         prev.build_smaller_level()
+    // }
+
+    // function method build_all_lpolys(): seq<lpolys>
+    // {
+
+    // }
+}
